examples/crypto/OPLSS.AE.fsti
@@ -14,34 +14,54 @@
    limitations under the License.
 *)
 module OPLSS.AE
-open OPLSS
-open FStar.Seq
-open FStar.HyperStack.ST
-module B = LowStar.Monotonic.Buffer
-module HS = FStar.HyperStack
+(* This is the interface for authenticated encryption (AE)
 
+   It provides an ideal view of AE in terms of a log associating
+   plain and ciphertexts.
+
+   However, this ideal interface is implemented without any loss in
+   security by composing secure interfaces for MACs (based on the
+   UF-CMA hypothesis) and Encryption (based on IND-CPA).
+*)
+open OPLSS //some basic definitions for this demo
+open FStar.Seq //F* library of sequences
+module HS = FStar.HyperStack //The memory model
+open FStar.HyperStack.ST //The State effect over that memory model
+module B = LowStar.Monotonic.Buffer //Arrays, abstract locations, framing etc.
+
+/// `key`: An abstract type of AE keys
 val key : Type u#0
 
-let ae_cipher = AES.iv_cipher * HMACSHA1.tag
+/// `ae_cipher`: An abstract type of AE ciphers
+val ae_cipher : eqtype
 
+/// The abstract memory footprint of key is just an abstract
+/// "location", i.e., `B.loc`
+///
+/// The function has effect `GTot`, meaning it is "Ghost" or
+/// computationally irrelevant, i.e., for specification only
 val footprint (k:key) : GTot B.loc
 
+/// We have an abstract invariant relating keys to memorys
 val invariant : key -> HS.mem -> prop
 
+/// Each element in the ae log associates a plain and a cipher text
 let log_entry = Plain.plain & ae_cipher
 
+/// ae_log: given a key and a memory (satisfying the invariant)
+/// we can (for spec purposes) read the log of entries
 val ae_log (k:key) (h:HS.mem{invariant k h})
   : GTot (Seq.seq log_entry)
 
 /// keygen: create a fresh key
-///         its ae log is initially empty
+///         When idealizing, its ae log is initially empty
 val keygen (_:unit)
   : ST key
   (requires fun _ -> True)
   (ensures  fun h0 k h1 ->
     B.modifies B.loc_none h0 h1 /\
     invariant k h1 /\
-    (Flag.reveal Ideal.uf_cma ==> ae_log k h1 == Seq.empty))
+    (Flag.reveal Ideal.ae ==> ae_log k h1 == Seq.empty))
 
 /// encrypt:
 ///       We return a cipher, preserve the invariant,
@@ -53,11 +73,12 @@ val encrypt (k:key) (plain:Plain.plain)
   (ensures  fun h0 c h1 ->
     invariant k h1 /\
     B.modifies (footprint k) h0 h1 /\
-    (Flag.reveal Ideal.uf_cma ==> ae_log k h1 == Seq.snoc (ae_log k h0) (plain, c)))
+    (Flag.reveal Ideal.ae ==> ae_log k h1 == Seq.snoc (ae_log k h0) (plain, c)))
 
 /// decrypt:
-///     In the ideal case, we prove it functionally correct and secure
-///     meaning that we the plain text returned is exactly the one in in AE log
+///     In the ideal case, we prove it functionally correct and
+///     secure meaning that the plain text returned is exactly the one
+///     in the AE log
 val decrypt (k:key) (c:ae_cipher)
   : ST (option Plain.plain)
   (requires
@@ -65,4 +86,4 @@ val decrypt (k:key) (c:ae_cipher)
   (ensures fun h0 res h1 ->
     invariant k h1 /\
     h0 == h1 /\
-    (Flag.reveal Ideal.uf_cma && Some? res ==> ae_log k h1 `Log.has` (Some?.v res, c)))
+    (Flag.reveal Ideal.ae && Some? res ==> ae_log k h1 `Log.has` (Some?.v res, c)))
