examples/crypto/OPLSS.fst
@@ -8,3 +8,17 @@ let lbytes l = b:bytes{Seq.length b = l}
 
 assume
 val random (l:nat) : EXT (lbytes l)
+
+assume
+val byte_of_int: n:nat{n < 256} -> Tot UInt8.t
+
+assume
+val xor: l:nat -> lbytes l -> lbytes l -> Tot (lbytes l)
+
+open FStar.Seq
+
+val auto_lemma_mem_snoc : #a:eqtype -> s:Seq.seq a -> x:a -> y:a ->
+   Lemma
+     (ensures (mem y (snoc s x) <==> mem y s \/ x=y))
+     [SMTPat (mem y (snoc s x))]
+let auto_lemma_mem_snoc #a s x y = Seq.lemma_mem_snoc s x
